# 条件

$$\begin{eqnarray}
条件: \quad
&①& \quad Euclid \ V\\
&②& \quad \mathscr{A}是\textcolor{pink}{\underline{\textbf{对称变换}}}
\end{eqnarray}$$
# 证明

$$\mathscr{A}的对应于\textcolor{orange}{\underline{\textbf{不同}}}的\textcolor{orange}{\underline{\textbf{特征值}}}\lambda_{1} \ , \ \lambda_{2}的\textcolor{orange}{\underline{\textbf{特征向量}}}\xi_{1} \ , \ \xi_{2}\textcolor{orange}{\underline{\textbf{互相正交}}}$$
$$\quad \Updownarrow \quad$$
$$(\xi_{1} \ , \ \xi_{2})=0 \quad \lambda_{1}  \ \neq \ \lambda_{2}$$
# Proof

因为

$$\mathscr{A}\xi_{1} = \lambda_{1} \xi_{1}$$
$$\mathscr{A}\xi_{2} = \lambda_{2}\xi_{2}$$
要证

$$(\xi_{1} \ , \ \xi_{2})=0$$
即证
$$\lambda_{1} (\xi_{1} \ , \ \xi_{2})=0$$
因为
$$\tag{*}\lambda_{1}(\xi_{1},\xi_{2})=(\lambda_{1} \xi_{1},\xi_{2})=(\mathscr{A}\xi_{1},\xi_{2})$$
又因为

$$\mathscr{A}是\textcolor{orange}{\underline{\textbf{对称变换}}}$$
$$\quad \Downarrow \quad $$
$$\tag{*}(\mathscr{A}\xi_{1},\xi_{2})=(\xi_{1},\mathscr{A}\xi_{2})=(\xi_{1},\lambda_{2}\xi_{2})=\lambda_{2}(\xi_{1},\xi_{2})$$
联立($*$)得

$$\lambda_{1}(\xi_{1},\xi_{2})=\lambda_{2}(\xi_{1},\xi_{2})$$
$$\quad \Downarrow \quad $$
$$(\lambda_{1}-\lambda_{2})(\xi_{1},\xi_{2})=0$$
因为
$$\lambda_{1}  \ \neq \  \lambda_{2}$$
$$\quad \Downarrow \quad $$
$$(\xi_{1},\xi_{2})=0 \qquad QED\ !$$

